Replace modules and functors with type classes (wip).
We can use type classes instead of modules and functors.
This way we avoid sharing constraints. Apparently, it is
inadvisable to use functors in Coq, so this is probably
a better option.

formalization/ett.v
@@ -1,7 +1,21 @@
+Require config.
 Require Import tt.
 
-Module Make (ConfigReflection : CONFIG_REFLECTION) :=
-  MakeEconomic(ConfigReflection).
+Section Ptt.
+
+Local Instance hasPrecond : config.Precond := {| config.precondFlag := config.No |}.
+Context `{configReflection : config.Reflection}.
+
+Definition isctx := isctx.
+Definition issubst := issubst.
+Definition istype := istype.
+Definition isterm := isterm.
+Definition eqctx := eqctx.
+Definition eqsubst := eqsubst.
+Definition eqtype := eqtype.
+Definition eqterm := eqterm.
+
+End Ptt.
 
 (* OLD STUFF BELOW
 
