formalization/config.v
@@ -1,0 +1,10 @@
+Class Precond := {
+  precondFlag : Type
+}.
+
+Class Reflection := {
+  reflectionFlag : Type
+}.
+
+Inductive Yes : Type := yes.
+Inductive No : Type := .
