formalization/config_tactics.v
@@ -1,54 +1,39 @@
-Require Import tt.
-
-Module Make
-       (ConfigPrecond : CONFIG_PRECOND)
-       (ConfigReflection : CONFIG_REFLECTION).
+Require Import config.
 
 (* Deal with configuration. *)
 Ltac doConfig :=
   (* configure the goal *)
   match goal with
-
-  (* Simplify the goal wrt preconditions *)
-  | |- (HasPrecond.precondFlag -> _) =>
-    (intros _)
-  | |- (HasntPrecond.precondFlag -> _) =>
-    let H := fresh "Eco" in
-    (intros H ; now elim H)
-  | |- (ConfigPrecond.precondFlag -> _) =>
-    let H := fresh "hasPrecond" in
-    (intros H)
-
-  (* Simplify the goal wrt reflection *)
-  | |- (HasReflection.reflectionFlag -> _) =>
-    (intros _)
-  | |- (HasntReflection.reflectionFlag -> _) =>
-    let H := fresh "Ref" in
-    (intros H ; now elim H)
-  | |- (ConfigReflection.reflectionFlag -> _) =>
-    let H := fresh "hasReflection" in
-    (intros H)
+  | |- ?P -> ?Q =>
+    match (eval cbv in P) with
+    | Yes => intros _
+    | No => let H := fresh "H" in (intros H ; now elim H)
+    | precondFlag =>
+      let H := fresh "precondFlag" in intros H
+    | reflectionFlag =>
+      let H := fresh "reflectionFlag" in intros H
+    | _ => idtac
+    end
   | _ => idtac
   end ;
-
   (* Configure the hypotheses *)
   repeat
   (match goal with
-
-   | H : HasPrecond.precondFlag -> ?A |- _ =>
-     apply (fun (f : HasPrecond.precondFlag -> A) => f HasPrecond.precond) in H
-   | H : HasntPrecond.precondFlag -> _ |- _ =>
-     clear H
-   | H : ConfigPrecond.precondFlag -> ?A, R : ConfigPrecond.precondFlag |- _ =>
-     apply (fun (f : ConfigPrecond.precondFlag -> A) => f R) in H
-
-   | H : HasReflection.reflectionFlag -> ?A |- _ =>
-     apply (fun (f : HasReflection.reflectionFlag -> A) => f HasReflection.reflection) in H
-   | H : HasntReflection.reflectionFlag -> _ |- _ =>
-     clear H
-   | H : ConfigReflection.reflectionFlag -> ?A, R : ConfigReflection.reflectionFlag |- _ =>
-     apply (fun (f : ConfigReflection.reflectionFlag -> A) => f R) in H
-   end).
+   | H : ?P -> ?Q |- _ =>
+     match (eval cbv in P) with
+     | Yes => specialize (H yes)
+     | No => clear H
+     | @precondFlag ?F =>
+       match goal with
+       | R : @precondFlag F |- _ => specialize (H R)
+       end
+     | @reflectionFlag ?F =>
+       match goal with
+       | R : @reflectionFlag F |- _ => specialize (H R)
+       end
+     end
+   | _ => idtac
+  end).
 
 (* Perform a tactic and deal with a configuration. *)
 Tactic Notation (at level 0) "config" tactic(t) := doConfig ; t ; doConfig.
@@ -56,5 +41,3 @@ Tactic Notation (at level 0) "config" tactic(t) := doConfig ; t ; doConfig.
 Tactic Notation (at level 5) "capply" uconstr(H) := doConfig ; apply H ; doConfig.
 
 Tactic Notation (at level 5) "ceapply" uconstr(H) := doConfig ; eapply H ; doConfig.
-
-End Make.
