formalization/ptt_sanity.v
@@ -1,19 +1,17 @@
 (* Sanity theorems for ptt. *)
 
+Require config.
+Require Import config_tactics.
+
 Require Import syntax.
-Require tt.
-Require ptt.
-Require config_tactics ptt_tactics ptt_admissible.
+Require Import tt.
+Require Import ptt_tactics ptt_admissible.
 
-Module Make (ConfigReflection : tt.CONFIG_REFLECTION).
+Section PttSanity.
 
-Module my_ptt_admissible := ptt_admissible.Make ConfigReflection.
-Import my_ptt_admissible.my_ptt_tactics.my_ptt.
-Import my_ptt_admissible.my_ptt_tactics.
-Import my_ptt_admissible.
+Local Instance hasPrecond : config.Precond := {| config.precondFlag := config.Yes |}.
+Context `{configReflection : config.Reflection}.
 
-Module my_config_tactics := config_tactics.Make tt.HasPrecond ConfigReflection.
-Import my_config_tactics.
 
 Definition sane_issubst sbs G D :
   issubst sbs G D -> isctx G * isctx D.
@@ -39,7 +37,7 @@ Proof.
 
     - capply CtxExtend.
       + assumption.
-      + now capply (@TySubst G D).
+      + now capply (@TySubst _ _ G D).
     - now capply CtxExtend.
   }
 
@@ -77,21 +75,21 @@ Proof.
   { config assumption. }
 
   (* TermCtxConv *)
-  { now capply (@TyCtxConv G D). }
+  { now capply (@TyCtxConv _ _ G D). }
 
   (* TermSubst *)
-  { now capply (@TySubst G D A sbs). }
+  { now capply (@TySubst _ _ G D A sbs). }
 
   (* TermVarZero *)
   { ceapply TySubst.
     - now ceapply SubstWeak.
     - assumption.
-    - now capply (@CtxExtend G A).
+    - now capply (@CtxExtend _ _ G A).
     - eassumption.
   }
 
   (* TermVarSucc *)
-  { capply (@TySubst (ctxextend G B) G).
+  { capply (@TySubst _ _ (ctxextend G B) G).
     - now capply SubstWeak.
     - assumption.
     - now capply CtxExtend.
@@ -102,7 +100,7 @@ Proof.
   { now capply (@TyProd). }
 
   (* TermApp *)
-  { capply (@TySubst G (ctxextend G A)).
+  { capply (@TySubst _ _ G (ctxextend G A)).
     - now capply SubstZero.
     - assumption.
     - assumption.
@@ -128,7 +126,7 @@ Proof.
   { now capply TyBool. }
 
   (* TermCond *)
-  { ceapply (@TySubst G (ctxextend G Bool)).
+  { ceapply (@TySubst _ _ G (ctxextend G Bool)).
     + config capply SubstZero.
       * assumption.
       * now capply TyBool.
@@ -157,8 +155,8 @@ Proof.
 
   (* EqTyCtxConv *)
   { split.
-    - { now capply (@TyCtxConv G D). }
-    - { now capply (@TyCtxConv G D). }
+    - { now capply (@TyCtxConv _ _ G D). }
+    - { now capply (@TyCtxConv _ _ G D). }
   }
 
   (* EqTyRefl*)
@@ -182,46 +180,46 @@ Proof.
 
   (* EqTySubstComp *)
   { split.
-    - capply (@TySubst G D) ; auto.
-      capply (@TySubst D E) ; auto.
-    - capply (@TySubst G E) ; auto.
-      capply (@SubstComp G D E) ; auto.
+    - capply (@TySubst _ _ G D) ; auto.
+      capply (@TySubst _ _ D E) ; auto.
+    - capply (@TySubst _ _ G E) ; auto.
+      capply (@SubstComp _ _ G D E) ; auto.
   }
 
   (* EqTySubstProd *)
   { split.
-    - { capply (@TySubst G D) ; auto using TyProd. }
+    - { capply (@TySubst _ _ G D) ; auto using TyProd. }
     - { capply TyProd ; auto.
-        + capply (@TySubst _ (ctxextend D A)) ; auto.
+        + capply (@TySubst _ _ _ (ctxextend D A)) ; auto.
           * now capply SubstShift.
           * capply CtxExtend ; auto.
-            now capply (@TySubst G D).
+            now capply (@TySubst _ _ G D).
           * now capply CtxExtend.
-        + now capply (@TySubst G D).
+        + now capply (@TySubst _ _ G D).
       }
   }
 
   (* EqTySubstId *)
   { split.
-    - { capply (@TySubst G D) ; auto using TyId. }
-    - { capply TyId ; auto using (@TySubst G D), (@TermSubst G D). }
+    - { capply (@TySubst _ _ G D) ; auto using TyId. }
+    - { capply TyId ; auto using (@TySubst _ _ G D), (@TermSubst _ _ G D). }
   }
 
   (* EqTySubstEmpty *)
   { split.
-    - { capply (@TySubst G D) ; auto using TyEmpty. }
+    - { capply (@TySubst _ _ G D) ; auto using TyEmpty. }
     - { now capply TyEmpty. }
   }
 
   (* EqTySubstUnit *)
   { split.
-    - { capply (@TySubst G D) ; auto using TyUnit. }
+    - { capply (@TySubst _ _ G D) ; auto using TyUnit. }
     - { now capply TyUnit. }
   }
 
   (* EqTySubstBool *)
   { split.
-    - { capply (@TySubst G D) ; auto using TyBool. }
+    - { capply (@TySubst _ _ G D) ; auto using TyBool. }
     - { now capply TyBool. }
   }
 
@@ -232,7 +230,7 @@ Proof.
   { split.
     - { now capply TyProd. }
     - { capply TyProd ; auto.
-        capply (@TyCtxConv (ctxextend G A1)) ; auto using CtxExtend.
+        capply (@TyCtxConv _ _ (ctxextend G A1)) ; auto using CtxExtend.
         capply EqCtxExtend ; auto using CtxRefl.
       }
   }
@@ -243,15 +241,15 @@ Proof.
     - { capply TyId.
         - assumption.
         - assumption.
-        - now capply (@TermTyConv G A B v1).
-        - now capply (@TermTyConv G A B v2).
+        - now capply (@TermTyConv _ _ G A B v1).
+        - now capply (@TermTyConv _ _ G A B v2).
       }
   }
 
   (* CongTySubst *)
   { split.
-    - { now capply (@TySubst G D). }
-    - { now capply (@TySubst G D). }
+    - { now capply (@TySubst _ _ G D). }
+    - { now capply (@TySubst _ _ G D). }
   }
 
 Defined.
@@ -290,7 +288,7 @@ Proof.
     - now capply CtxExtend.
     - capply CtxExtend.
       + assumption.
-      + capply (@TyCtxConv G D) ; auto.
+      + capply (@TyCtxConv _ _ G D) ; auto.
   }
 
 Defined.
@@ -330,12 +328,12 @@ Proof.
   (* CongSubstZero *)
   - { split.
       - now capply SubstZero.
-      - capply (@SubstCtxConv G G (ctxextend G A2) (ctxextend G A1)) ;
+      - capply (@SubstCtxConv _ _ G G (ctxextend G A2) (ctxextend G A1)) ;
           auto using CtxExtend, CtxRefl, CtxSym.
         + capply SubstZero ;
-            auto using (@TyCtxConv G G), (@TermCtxConv G G), (@TermTyConv G A1 A2).
+            auto using (@TyCtxConv _ _ G G), (@TermCtxConv _ _ G G), (@TermTyConv _ _ G A1 A2).
         + capply EqCtxExtend ;
-            auto using (@TyCtxConv G G), CtxRefl, (@EqTyCtxConv G G), EqTySym.
+            auto using (@TyCtxConv _ _ G G), CtxRefl, (@EqTyCtxConv _ _ G G), EqTySym.
     }
 
   (* CongSubstWeak *)
@@ -346,74 +344,74 @@ Proof.
 
   (* CongSubstComp *)
   - { split.
-      - now capply (@SubstComp G D E).
-      - now capply (@SubstComp G D E).
+      - now capply (@SubstComp _ _ G D E).
+      - now capply (@SubstComp _ _ G D E).
     }
 
   (* EqSubstCtxConv *)
   - { split.
-      - now capply (@SubstCtxConv G1 G2 D1 D2).
-      - now capply (@SubstCtxConv G1 G2 D1 D2).
+      - now capply (@SubstCtxConv _ _ G1 G2 D1 D2).
+      - now capply (@SubstCtxConv _ _ G1 G2 D1 D2).
     }
 
   (* CompAssoc *)
   - { split.
-      - capply (@SubstComp G E F) ; auto.
-        now capply (@SubstComp G D E).
-      - capply (@SubstComp G D F); auto.
-        now capply (@SubstComp D E F).
+      - capply (@SubstComp _ _ G E F) ; auto.
+        now capply (@SubstComp _ _ G D E).
+      - capply (@SubstComp _ _ G D F); auto.
+        now capply (@SubstComp _ _ D E F).
     }
 
   (* WeakNat *)
   - { split.
-      - capply (@SubstComp _ (ctxextend D A)) ;
-          auto using CtxExtend, (@TySubst G D), SubstShift, SubstWeak.
-      - capply (@SubstComp _ G) ;
-          auto using CtxExtend, (@TySubst G D), SubstWeak.
+      - capply (@SubstComp _ _ _ (ctxextend D A)) ;
+          auto using CtxExtend, (@TySubst _ _ G D), SubstShift, SubstWeak.
+      - capply (@SubstComp _ _ _ G) ;
+          auto using CtxExtend, (@TySubst _ _ G D), SubstWeak.
     }
 
   (* WeakZero *)
   - { split.
-      - capply (@SubstComp _ (ctxextend G A)) ;
+      - capply (@SubstComp _ _ _ (ctxextend G A)) ;
           auto using CtxExtend, SubstZero, SubstWeak.
       - now capply SubstId.
     }
 
   (* ShiftZero *)
   - { split.
-      - capply (@SubstComp _ (ctxextend G (Subst A sbs))) ;
-          auto using CtxExtend, (@TySubst G D), SubstZero, (@TermSubst G D), SubstShift.
-      - capply (@SubstComp _ D) ;
+      - capply (@SubstComp _ _ _ (ctxextend G (Subst A sbs))) ;
+          auto using CtxExtend, (@TySubst _ _ G D), SubstZero, (@TermSubst _ _ G D), SubstShift.
+      - capply (@SubstComp _ _ _ D) ;
           auto using CtxExtend, SubstZero.
     }
 
   (* CompShift *)
   - { split.
-      - capply (@SubstComp _ (ctxextend D (Subst A sbt))) ;
-          auto using CtxExtend, (@TySubst D E), SubstShift.
-        + { capply (@SubstCtxConv (ctxextend G (Subst (Subst A sbt) sbs)) _
+      - capply (@SubstComp _ _ _ (ctxextend D (Subst A sbt))) ;
+          auto using CtxExtend, (@TySubst _ _ D E), SubstShift.
+        + { capply (@SubstCtxConv _ _ (ctxextend G (Subst (Subst A sbt) sbs)) _
                                  (ctxextend D (Subst A sbt))) ;
-            auto using CtxExtend, (@TySubst D E), (@TySubst G D), (@TySubst G E),
-                       (@SubstComp G D E), SubstShift, CtxRefl.
+            auto using CtxExtend, (@TySubst _ _ D E), (@TySubst _ _ G D), (@TySubst _ _ G E),
+                       (@SubstComp _ _ G D E), SubstShift, CtxRefl.
             capply EqCtxExtend ;
-                auto using CtxRefl, (@TySubst G D), (@TySubst D E),
-                           (@TySubst G E), (@SubstComp G D E).
-              now capply (@EqTySubstComp G D E).
+                auto using CtxRefl, (@TySubst _ _ G D), (@TySubst _ _ D E),
+                           (@TySubst _ _ G E), (@SubstComp _ _ G D E).
+              now capply (@EqTySubstComp _ _ G D E).
           }
         + capply CtxExtend ; auto.
-          capply (@TySubst G E) ; auto using (@SubstComp G D E).
-      - capply SubstShift ; auto using (@SubstComp G D E).
+          capply (@TySubst _ _ G E) ; auto using (@SubstComp _ _ G D E).
+      - capply SubstShift ; auto using (@SubstComp _ _ G D E).
     }
 
   (* CompIdRight *)
   - { split.
-      - capply (@SubstComp G G D) ; auto using SubstId.
+      - capply (@SubstComp _ _ G G D) ; auto using SubstId.
       - assumption.
     }
 
   (* CompIdLeft *)
   - { split.
-      - capply (@SubstComp G D D) ; auto using SubstId.
+      - capply (@SubstComp _ _ G D D) ; auto using SubstId.
       - assumption.
     }
 Defined.
@@ -433,14 +431,14 @@ Proof.
 
   (* EqTyConv *)
   - { split.
-      - { now capply (@TermTyConv G A B u). }
-      - { now capply (@TermTyConv G A B v). }
+      - { now capply (@TermTyConv _ _ G A B u). }
+      - { now capply (@TermTyConv _ _ G A B v). }
     }
 
   (* EqCtxConv *)
   - { split.
-      - { now capply (@TermCtxConv G D A). }
-      - { now capply (@TermCtxConv G D A). }
+      - { now capply (@TermCtxConv _ _ G D A). }
+      - { now capply (@TermCtxConv _ _ G D A). }
     }
 
   (* EqRefl *)
@@ -463,11 +461,11 @@ Proof.
 
   (* EqIdSubst *)
   - { split.
-      - { capply (@TermTyConv G (Subst A sbid) A).
-          - capply (@TermSubst G G) ; auto using SubstId.
+      - { capply (@TermTyConv _ _ G (Subst A sbid) A).
+          - capply (@TermSubst _ _ G G) ; auto using SubstId.
           - now capply EqTyIdSubst.
           - assumption.
-          - capply (@TySubst G G) ; auto using SubstId.
+          - capply (@TySubst _ _ G G) ; auto using SubstId.
           - assumption.
         }
       - { assumption. }
@@ -475,25 +473,25 @@ Proof.
 
   (* EqSubstComp *)
   - { split.
-      - { capply (@TermTyConv G (Subst (Subst A sbt) sbs) (Subst A (sbcomp sbt sbs))).
-          - capply (@TermSubst G D) ; auto.
-            + now capply (@TermSubst D E).
-            + now capply (@TySubst D E).
-          - now capply (@EqTySubstComp G D E).
+      - { capply (@TermTyConv _ _ G (Subst (Subst A sbt) sbs) (Subst A (sbcomp sbt sbs))).
+          - capply (@TermSubst _ _ G D) ; auto.
+            + now capply (@TermSubst _ _ D E).
+            + now capply (@TySubst _ _ D E).
+          - now capply (@EqTySubstComp _ _ G D E).
           - assumption.
-          - capply (@TySubst G D) ; auto.
-            now capply (@TySubst D E).
-          - capply (@TySubst G E) ; auto.
-            now capply (@SubstComp G D E).
+          - capply (@TySubst _ _ G D) ; auto.
+            now capply (@TySubst _ _ D E).
+          - capply (@TySubst _ _ G E) ; auto.
+            now capply (@SubstComp _ _ G D E).
         }
-      - { capply (@TermSubst G E) ; auto.
-          now capply (@SubstComp G D E).
+      - { capply (@TermSubst _ _ G E) ; auto.
+          now capply (@SubstComp _ _ G D E).
         }
     }
 
   (* EqSubstWeak *)
   - { split.
-      - { capply (@TermSubst _ G) ; auto using CtxExtend.
+      - { capply (@TermSubst _ _ _ G) ; auto using CtxExtend.
           now capply SubstWeak.
         }
       - { now capply TermVarSucc. }
@@ -502,32 +500,32 @@ Proof.
 
   (* EqSubstZeroZero *)
   - { split.
-      - { capply (@TermTyConv G (Subst (Subst A (sbweak A)) (sbzero A u))).
-          - capply (@TermSubst _ (ctxextend G A)) ; auto using CtxExtend.
+      - { capply (@TermTyConv _ _ G (Subst (Subst A (sbweak A)) (sbzero A u))).
+          - capply (@TermSubst _ _ _ (ctxextend G A)) ; auto using CtxExtend.
             + now capply SubstZero.
             + now capply TermVarZero.
-            + capply (@TySubst _ G) ; auto using CtxExtend, SubstWeak.
-          - capply (@EqTyTrans G _ (Subst A sbid)) ; auto.
-            + { capply (@EqTyTrans _ _ (Subst A (sbcomp (sbweak A) (sbzero A u)))) ; auto.
-                - capply (@EqTySubstComp G (ctxextend G A) G) ;
-                    auto using CtxExtend, (@SubstComp G (ctxextend G A)) , SubstWeak, SubstZero.
-                - capply (@CongTySubst G G) ;
-                    auto using CtxExtend, (@SubstComp G (ctxextend G A)) , SubstWeak, SubstZero, SubstId, EqTyRefl, WeakZero.
-                - capply (@TySubst _ (ctxextend G A)) ; auto using CtxExtend, SubstZero.
-                  capply (@TySubst _ G) ; auto using CtxExtend, SubstWeak.
-                - capply (@TySubst _ G) ; auto.
-                  + capply (@SubstComp _ (ctxextend G A)) ; auto using CtxExtend, SubstWeak, SubstZero.
-                - capply (@TySubst _ G) ; auto using SubstId.
+            + capply (@TySubst _ _ _ G) ; auto using CtxExtend, SubstWeak.
+          - capply (@EqTyTrans _ _ G _ (Subst A sbid)) ; auto.
+            + { capply (@EqTyTrans _ _ _ _ (Subst A (sbcomp (sbweak A) (sbzero A u)))) ; auto.
+                - capply (@EqTySubstComp _ _ G (ctxextend G A) G) ;
+                    auto using CtxExtend, (@SubstComp _ _ G (ctxextend G A)) , SubstWeak, SubstZero.
+                - capply (@CongTySubst _ _ G G) ;
+                    auto using CtxExtend, (@SubstComp _ _ G (ctxextend G A)) , SubstWeak, SubstZero, SubstId, EqTyRefl, WeakZero.
+                - capply (@TySubst _ _ _ (ctxextend G A)) ; auto using CtxExtend, SubstZero.
+                  capply (@TySubst _ _ _ G) ; auto using CtxExtend, SubstWeak.
+                - capply (@TySubst _ _ _ G) ; auto.
+                  + capply (@SubstComp _ _ _ (ctxextend G A)) ; auto using CtxExtend, SubstWeak, SubstZero.
+                - capply (@TySubst _ _ _ G) ; auto using SubstId.
               }
             + now capply EqTyIdSubst.
-            + capply (@TySubst _ (ctxextend G A)) ; auto using CtxExtend.
+            + capply (@TySubst _ _ _ (ctxextend G A)) ; auto using CtxExtend.
               * now capply SubstZero.
-              * capply (@TySubst _ G) ; auto using CtxExtend, SubstWeak.
-            + capply (@TySubst _ G) ; auto using SubstId.
+              * capply (@TySubst _ _ _ G) ; auto using CtxExtend, SubstWeak.
+            + capply (@TySubst _ _ _ G) ; auto using SubstId.
           - assumption.
-          - capply (@TySubst _ (ctxextend G A)) ; auto using CtxExtend.
+          - capply (@TySubst _ _ _ (ctxextend G A)) ; auto using CtxExtend.
             + now capply SubstZero.
-            + capply (@TySubst _ G) ; auto using CtxExtend.
+            + capply (@TySubst _ _ _ G) ; auto using CtxExtend.
               now capply SubstWeak.
           - assumption.
         }
@@ -536,15 +534,15 @@ Proof.
 
   (* EqSubstZeroSucc *)
   - { split.
-      - { capply (@TermTyConv G (Subst (Subst A (sbweak B)) (sbzero B u))).
-          - capply (@TermSubst G (ctxextend G B)) ; auto using CtxExtend.
+      - { capply (@TermTyConv _ _ G (Subst (Subst A (sbweak B)) (sbzero B u))).
+          - capply (@TermSubst _ _ G (ctxextend G B)) ; auto using CtxExtend.
             + now capply SubstZero.
             + now capply TermVarSucc.
-            + capply (@TySubst _ G) ; auto using CtxExtend, SubstWeak.
+            + capply (@TySubst _ _ _ G) ; auto using CtxExtend, SubstWeak.
           - capply EqTySym ; magic.
           - assumption.
-          - capply (@TySubst _ (ctxextend G B)) ; auto using CtxExtend, SubstZero.
-            capply (@TySubst _ G) ; auto using CtxExtend, SubstWeak.
+          - capply (@TySubst _ _ _ (ctxextend G B)) ; auto using CtxExtend, SubstZero.
+            capply (@TySubst _ _ _ G) ; auto using CtxExtend, SubstWeak.
           - assumption.
         }
       - { assumption. }
@@ -745,4 +743,4 @@ Proof.
   auto using (@sane_isterm G u A).
 Defined.
 
-End Make.
+End PttSanity.
